Impl gensyms

theories/L6_PCPS/uncurry_proto.v
@@ -1,7 +1,7 @@
 (** Uncurrying written as a guarded rewrite rule *)
 
 Require Import Coq.Strings.String.
-Require Import Coq.NArith.BinNat Coq.PArith.BinPos Coq.Sets.Ensembles Omega.
+Require Import Coq.NArith.BinNat Coq.PArith.BinPos Coq.Sets.Ensembles micromega.Lia.
 Require Import L6.Prototype.
 Require Import L6.cps_proto.
 Require Import identifiers.  (* for max_var, occurs_in_exp, .. *)
@@ -64,9 +64,10 @@ Proof. constructor. Defined.
 Instance Preserves_S_S : Preserves_S _ exp_univ_exp (@S).
 Proof. constructor; intros; assumption. Defined.
 
-Definition fresh_copies (S : Ensemble cps.var) (l : list cps.var) : Prop :=
-  Disjoint _ S (FromList l) /\ NoDup l.
+Definition fresh_copies (S : Ensemble cps.var) (l : list var) : Prop :=
+  Disjoint _ S (FromList ![l]) /\ NoDup l.
 
+(* Uncurrying as a guarded rewrite rule *)
 Inductive uncurry_step : exp -> exp -> Prop :=
 | uncurry_cps :
   forall (C : frames_t exp_univ_fundefs exp_univ_exp)
@@ -86,14 +87,14 @@ Inductive uncurry_step : exp -> exp -> Prop :=
   rhs = Fcons f ft (k :: fv1) (Efun (Fcons g gt gv1 (Eapp f1 ft1 (gv1 ++ fv1)) Fnil) (Eapp k kt [g]))
         (Fcons f1 ft1 (gv ++ fv) ge (Rec fds)) /\
   s = used_vars (exp_of_proto (C ⟦ lhs ⟧)) /\
-  fresh_copies s ![gv1] -> length gv1 = length gv /\
-  fresh_copies (s :|: FromList ![gv1]) ![fv1] -> length fv1 = length fv /\
+  fresh_copies s gv1 -> length gv1 = length gv /\
+  fresh_copies (s :|: FromList ![gv1]) fv1 -> length fv1 = length fv /\
   ~ ![f1] \in (s :|: FromList ![gv1] :|: FromList ![fv1]) /\
   (* (3) next_x must be a fresh variable *)
   fresher_than next_x (s :|: FromList ![gv1] :|: FromList ![fv1]) /\
   (* (4) ft1 is the appropriate fun_tag and ms is an updated misc state. *)
   fp_numargs = length fv + length gv /\
-  (let '(_, aenv, _, _) := ms in PM.get ![ft1] aenv <> None) -> (* TODO: proper side condition *)
+  (True \/ let '(_, aenv, _, _) := ms in PM.get ![ft1] aenv <> None) -> (* TODO: proper side condition *)
   (* 'Irrelevant' guard *)
   When (fun (r : R_misc) (s : S_misc) =>
     let '(b, aenv, lm, s) := s in
@@ -118,6 +119,80 @@ Inductive uncurry_step : exp -> exp -> Prop :=
          (Fcons f ft (k :: fv1) (Efun (Fcons g gt gv1 (Eapp f1 ft1 (gv1 ++ fv1)) Fnil) (Eapp k kt [g]))
          (Fcons f1 ft1 (gv ++ fv) ge (Rec fds))) ⟧).
 
+Fixpoint gensyms {A} (x : cps.var) (xs : list A) : cps.var * list var :=
+  match xs with
+  | [] => (x, [])
+  | _ :: xs => let '(x', xs') := gensyms (1 + x)%positive xs in (x', mk_var x :: xs')
+  end.
+
+Lemma gensyms_len {A} x (xs : list A) : length (snd (gensyms x xs)) = length xs.
+Proof.
+  revert x; induction xs; auto; intros.
+  unfold gensyms; fold @gensyms; destruct (gensyms _ _) as [x' xs'] eqn:Hxs'; simpl.
+  now erewrite <- IHxs, Hxs'.
+Qed.
+
+Local Ltac mk_corollary parent := 
+  intros x xs x' xs';
+  pose (Hparent := parent _ x xs); clearbody Hparent; intros H;
+  destruct (gensyms x xs); now inversion H.
+
+Corollary gensyms_len' {A} : forall x (xs : list A) x' xs', (x', xs') = gensyms x xs -> length xs' = length xs.
+Proof. mk_corollary @gensyms_len. Qed.
+
+Lemma gensyms_increasing {A} x (xs : list A) : forall y, List.In y (snd (gensyms x xs)) -> (![y] >= x)%positive.
+Proof.
+  revert x; induction xs; [now simpl|intros x [y] Hy].
+  unfold gensyms in Hy; fold @gensyms in Hy.
+  destruct (gensyms _ _) as [x' xs'] eqn:Hxs'.
+  simpl in Hy; destruct Hy as [H|H]; [inversion H; simpl; lia|].
+  specialize (IHxs (1 + x)%positive (mk_var y)).
+  rewrite Hxs' in IHxs; unfold snd in IHxs.
+  specialize (IHxs H); lia.
+Qed.
+
+Lemma gensyms_upper {A} x (xs : list A) :
+  (fst (gensyms x xs) >= x)%positive /\
+  forall y, List.In y (snd (gensyms x xs)) -> (fst (gensyms x xs) > ![y])%positive.
+Proof.
+  revert x; induction xs; [simpl; split; [lia|easy]|intros x; split; [|intros [y] Hy]].
+  - unfold gensyms; fold @gensyms.
+    destruct (gensyms _ _) as [x' xs'] eqn:Hxs'; unfold fst.
+    specialize (IHxs (1 + x)%positive); rewrite Hxs' in IHxs; unfold fst in IHxs.
+    destruct IHxs; lia.
+  - unfold gensyms in *; fold @gensyms in *.
+    destruct (gensyms _ _) as [x' xs'] eqn:Hxs'; unfold fst; unfold snd in Hy.
+    specialize (IHxs (1 + x)%positive); rewrite Hxs' in IHxs; unfold fst in IHxs.
+    destruct IHxs as [IHxs IHxsy].
+    destruct Hy as [Hy|Hy]; [inversion Hy; simpl; lia|].
+    now specialize (IHxsy (mk_var y) Hy).
+Qed.
+
+Lemma gensyms_NoDup {A} x (xs : list A) : NoDup (snd (gensyms x xs)).
+Proof.
+  revert x; induction xs; intros; [now constructor|].
+  unfold gensyms; fold @gensyms.
+  destruct (gensyms _ _) as [x' xs'] eqn:Hxs'; unfold snd.
+  specialize (IHxs (1 + x)%positive); rewrite Hxs' in IHxs; unfold snd in IHxs.
+  constructor; [|auto].
+  pose (Hinc := gensyms_increasing (1 + x)%positive xs); clearbody Hinc.
+  rewrite Hxs' in Hinc; unfold snd in Hinc.
+  remember (snd (gensyms (1 + x)%positive xs)) as ys; clear - Hinc.
+  induction xs'; auto.
+  intros [|Hin_ys]; [|apply IHxs'; auto; intros; apply Hinc; now right].
+  assert (Hxa : In (mk_var x) (a :: xs')) by now left.
+  specialize (Hinc (mk_var x) Hxa); unfold isoBofA, Iso_var, un_var in Hinc; lia.
+Qed.
+
+Corollary gensyms_NoDup' {A} : forall x (xs : list A) x' xs', (x', xs') = gensyms x xs -> NoDup xs'.
+Proof. mk_corollary @gensyms_NoDup. Qed.
+
+Lemma bool_true_false b : b = false -> b <> true. Proof. now destruct b. Qed.
+
+Local Ltac clearpose H x e :=
+  pose (x := e); assert (H : x = e) by (subst x; reflexivity); clearbody x.
+
+(* Uncurrying as a recursive function *)
 Definition rw_cp : rewriter exp_univ_exp uncurry_step R_misc S_misc (@delay_t) (@R_C) (@R_e) (@S).
 Proof.
   mk_rw;
@@ -138,26 +213,40 @@ Proof.
     destruct (eq_var g g') eqn:Hgg'; [|exact failure].
     rewrite Pos.eqb_eq in Hkk', Hgg'.
     (* Check whether g has already been uncurried before *)
-    destruct ms as [[[b aenv] lm] heuristic].
+    destruct ms as [[[b aenv] lm] heuristic] eqn:Hms.
     destruct (PM.get g lm) as [[|]|] eqn:Huncurried; [|exact failure..].
     (* Check that {g, k} ∩ vars(ge) = ∅ *)
-    destruct (occurs_in_exp g ![ge]) eqn:Hocc_g; [|exact failure]. (* TODO: avoid the conversion *)
-    destruct (occurs_in_exp k ![ge]) eqn:Hocc_k; [|exact failure]. (* TODO: avoid the conversion *)
+    destruct (occurs_in_exp g ![ge]) eqn:Hocc_g; [exact failure|]. (* TODO: avoid the conversion *)
+    destruct (occurs_in_exp k ![ge]) eqn:Hocc_k; [exact failure|]. (* TODO: avoid the conversion *)
+    apply bool_true_false in Hocc_g; apply bool_true_false in Hocc_k.
     rewrite occurs_in_exp_iff_used_vars in Hocc_g, Hocc_k.
     (* Generate ft1 + new misc state ms *)
     idtac "TODO: generate ft1 and new misc state ms".
+    specialize success with (ft1 := mk_fun_tag xH). (* Until comp_data : Set, put some bogus stuff *)
+    specialize success with (ms := ms).
     (* Generate f1, fv1, gv1, next_x *)
-    idtac "TODO: generate f1, ft1, fv1, gv1, next_x".
-    (* Prove that the freshly generated names are actually fresh *)
-    idtac "TODO: vars proof".
-    admit.
+    destruct s as [next_x Hnext_x].
+    clearpose Hxgv1 xgv1 (gensyms next_x gv); destruct xgv1 as [next_x0 gv1].
+    clearpose Hxfv1 xfv1 (gensyms next_x0 fv); destruct xfv1 as [next_x1 fv1].
+    clearpose Hf1 f1 next_x1.
+    (* Prove that all the above code actually satisfies the side conditions *)
+    eapply success with (f1 := mk_var f1) (fv1 := fv1) (gv1 := gv1) (next_x := (next_x1 + 1)%positive);
+      repeat match goal with |- _ /\ _ => split | |- fresh_copies _ _ => split end; try solve
+      [reflexivity|assumption|subst;reflexivity
+      |eapply gensyms_NoDup'; eassumption
+      |eapply gensyms_len'; eassumption].
+    + admit.
+    + admit.
+    + admit.
+    + admit.
+    + admit.
+    + destruct (Maps.PTree.get _ _) as [[|]|] eqn:Hget'; [reflexivity|inversion Huncurried..].
   (* Obligation 2 of 2: explain how to maintain fresh name invariant across edit *)
-  - clear; intros.
+  - clear; unfold Put, Rec; intros.
     (* Env is easy, because the uncurryer doesn't need it *)
     split; [exact tt|].
     (* For state, need create a fresh variable. Thankfully, we have one: next_x *)
-    exists next_x; unfold Put, Rec.
-    repeat match goal with H : _ /\ _ |- _ => destruct H end.
+    exists next_x; repeat match goal with H : _ /\ _ |- _ => destruct H end.
     eapply fresher_than_antimon; [|eassumption].
     admit.
 Admitted.
